examples/map/MapA.v
@@ -83,13 +83,7 @@ Section A.
   .
 
   Variable GlobalStb: Sk.t -> gname -> option fspec.
-  Definition _t: HMod.t := (SMod.to_hmod GlobalStb Mod).
-  Definition t := _t.
-
-  Lemma unfold: t = _t.
-  Proof. eauto. Qed.
-
-  Global Opaque t.
+  Definition t := Seal.sealing "ccr" (SMod.to_hmod GlobalStb Mod).
 
 End A.
 End MapA.
