examples/ring/RingIAproof.v
@@ -43,8 +43,6 @@ Definition HMod_empty: HMod.t :=
 End XXX.
 
 
-  
-
 Module RingIA.
 Section SIMMODSEM.
   Context `{Σ: GRA.t}.
@@ -70,114 +68,91 @@ Section SIMMODSEM.
   
   Local Notation RingIMod := (HMod.add CtrlIMod (CellGroup max_size)).
 
-  Definition rotate_rev {T} n (l: list T) :=
-    drop ((strings.length l)-(n mod strings.length l)) l ++ take ((strings.length l)-(n mod strings.length l)) l.
+(*   Variable fl: alist string (Any.t → itree hmodE Any.t). *)
+(*   Variable fr: alist string (Any.t → itree hmodE Any.t). *)
 
-  Lemma rotate_rev_inv {T} n (l: list T):
-    rotate_rev n (rotate n l) = l.
-  Proof. admit. Admitted.
+(* Ltac init_simF := let name := fresh "name" in *)
+(*   unfold HModR.sim_fun; i; *)
+(*   do 2 match goal with *)
+(*   | [|-context[alist_find _ (_ (_ (HMod.add ?x _) _))]] => rewrite/__ {1}/x *)
+(*   | [|-context[alist_find _ (_ (_ ?x _))]] => rewrite/__ {1}/x *)
+(*   end; *)
+(*   unseal "ccr"; *)
+(*   alist_find_solver; *)
+(*   repeat match goal with *)
+(*   | [|- context[{| fsb_body := cfunU ?x |}]] => rewrite/__ {1}/x *)
+(*   | [|- context[cfunU ?x]] => rewrite/__ {1}/x *)
+(*   end; *)
+(*   unfold interp_sb_hp, HoareFun, cfunU, ccallU; s; *)
+(*   ii; subst; iIntros "IST". *)
 
-  Lemma rotate_rev_id {T} (l: list T):
-    rotate_rev 0 l = l.
-  Proof. admit. Admitted.
-  
-  Definition Ist: Any.t -> Any.t -> iProp :=
-    (fun st_src st_tgt =>
-       ((∃ (sz:nat) (q q': list Z) (hd tl: nat) cell_state,
-         ⌜st_src = (sz, q)↑ /\ List.length q = sz /\ sz < max_size /\
-          st_tgt = Any.pair (hd,tl)↑ cell_state /\ hd-tl = sz /\
-          List.length (q ++ q') = max_size⌝ ∗
-          [∗ list] i↦x ∈ rotate_rev tl (q++q'), (CellAS.pending i ∨ CellAS.cell (i mod max_size) x))))%I.
+(* Ltac hss := *)
+(*   ss; *)
+(*   try (unfold run_l, run_r in *; rewrite !Any.pair_split in *; fold run_l run_r in * ); *)
+(*   try (rewrite !Any.upcast_downcast in * ); *)
+(*   (repeat match goal with [G: Any.downcast _ = Some _ |-_] => *)
+(*     apply Any.downcast_upcast in G; inv G; ss *)
+(*    end); *)
+(*   (repeat match goal with [G: Any.upcast (_:?T) = Any.upcast (_:?T) |-_] => *)
+(*     apply Any.upcast_inj in G; destruct G as [_ G]; red in G; depdes G; ss *)
+(*    end); *)
+(*   (repeat match goal with [G: Some _ = Some _ |- _] => *)
+(*     depdes G; ss *)
+(*    end). *)
 
-  Variable fl: alist string (Any.t → itree hmodE Any.t).
-  Variable fr: alist string (Any.t → itree hmodE Any.t).
+(* Ltac inv_string X := *)
+(*   inv X; *)
+(*   repeat match goal with [H: @eq string (_ ++ _)%string (_ ++ _)%string|-_] => *)
+(*            apply string_app_inv in H *)
+(*     end; ss. *)
 
-Ltac init_simF := let name := fresh "name" in
-  unfold HModR.sim_fun; i;
-  do 2 match goal with
-  | [|-context[alist_find _ (_ (_ (HMod.add ?x _) _))]] => rewrite/__ {1}/x
-  | [|-context[alist_find _ (_ (_ ?x _))]] => rewrite/__ {1}/x
-  end;
-  unseal "ccr";
-  alist_find_solver;
-  repeat match goal with
-  | [|- context[{| fsb_body := cfunU ?x |}]] => rewrite/__ {1}/x
-  | [|- context[cfunU ?x]] => rewrite/__ {1}/x
-  end;
-  unfold interp_sb_hp, HoareFun, cfunU, ccallU; s;
-  ii; subst; iIntros "IST".
+(* Ltac alist_find_solver := *)
+(*   match goal with [|-context[alist_find ?x]] => rewrite <-(Seal.sealing_eq "_tmp_" x) end; *)
+(*   s; unfold rel_dec, Dec_RelDec, sumbool_to_bool, dec, string_Dec; *)
+(*   des_ifs; unseal "_tmp_"; *)
+(*   repeat match goal with [H: @eq string _ _|-_] => inv_string H end; *)
+(*   repeat match goal with [H: not (@eq string _ _)|-_] => clear H end. *)
 
-Ltac hss :=
-  ss;
-  try (unfold run_l, run_r in *; rewrite !Any.pair_split in *; fold run_l run_r in * );
-  try (rewrite !Any.upcast_downcast in * );
-  (repeat match goal with [G: Any.downcast _ = Some _ |-_] =>
-    apply Any.downcast_upcast in G; inv G; ss
-   end);
-  (repeat match goal with [G: Any.upcast (_:?T) = Any.upcast (_:?T) |-_] =>
-    apply Any.upcast_inj in G; destruct G as [_ G]; red in G; depdes G; ss
-   end);
-  (repeat match goal with [G: Some _ = Some _ |- _] =>
-    depdes G; ss
-   end).
+(* Lemma string_app_length s1 s2: *)
+(*   length (s1++s2)%string = length s1 + length s2. *)
+(* Proof. *)
+(*   induction s1. *)
+(*   - unfold append; fold append. eauto. *)
+(*   - s. fold append. rewrite IHs1. nia. *)
+(* Qed. *)
 
-Ltac inv_string X :=
-  inv X;
-  repeat match goal with [H: @eq string (_ ++ _)%string (_ ++ _)%string|-_] =>
-           apply string_app_inv in H
-    end; ss.
+(* Lemma string_app_inv_r *)
+(*   p s s' *)
+(*   (EQ: (s ++ p = s' ++ p)%string) *)
+(*   : *)
+(*   (s = s')%string. *)
+(* Proof. *)
+(*   revert p s' EQ. induction s; i; ss. *)
+(*   { destruct s'; eauto. *)
+(*     apply (f_equal length) in EQ. *)
+(*     rewrite !string_app_length in EQ. ss. nia. } *)
+(*   destruct s'. *)
+(*   { apply (f_equal length) in EQ. *)
+(*     rewrite !string_app_length in EQ. ss. nia. } *)
+(*   revert EQ. unfold append; fold append. i. *)
+(*   inv EQ. f_equal. eauto. *)
+(* Qed. *)
 
-Ltac alist_find_solver :=
-  match goal with [|-context[alist_find ?x]] => rewrite <-(Seal.sealing_eq "_tmp_" x) end;
-  s; unfold rel_dec, Dec_RelDec, sumbool_to_bool, dec, string_Dec;
-  des_ifs; unseal "_tmp_";
-  repeat match goal with [H: @eq string _ _|-_] => inv_string H end;
-  repeat match goal with [H: not (@eq string _ _)|-_] => clear H end.
+(* Lemma list_ascii_of_string_app s1 s2: *)
+(*   list_ascii_of_string (s1 ++ s2)%string = *)
+(*     list_ascii_of_string s1 ++ list_ascii_of_string s2. *)
+(* Proof. *)
+(*   revert s2. induction s1; i; s; eauto. *)
+(*   rewrite IHs1; eauto. *)
+(* Qed. *)
 
-
-
-
-
-Lemma string_app_length s1 s2:
-  length (s1++s2)%string = length s1 + length s2.
-Proof.
-  induction s1.
-  - unfold append; fold append. eauto.
-  - s. fold append. rewrite IHs1. nia.
-Qed.
-
-Lemma string_app_inv_r
-  p s s'
-  (EQ: (s ++ p = s' ++ p)%string)
-  :
-  (s = s')%string.
-Proof.
-  revert p s' EQ. induction s; i; ss.
-  { destruct s'; eauto.
-    apply (f_equal length) in EQ.
-    rewrite !string_app_length in EQ. ss. nia. }
-  destruct s'.
-  { apply (f_equal length) in EQ.
-    rewrite !string_app_length in EQ. ss. nia. }
-  revert EQ. unfold append; fold append. i.
-  inv EQ. f_equal. eauto.
-Qed.
-
-Lemma list_ascii_of_string_app s1 s2:
-  list_ascii_of_string (s1 ++ s2)%string =
-    list_ascii_of_string s1 ++ list_ascii_of_string s2.
-Proof.
-  revert s2. induction s1; i; s; eauto.
-  rewrite IHs1; eauto.
-Qed.
-
-Lemma string_of_list_ascii_app l1 l2:
-  string_of_list_ascii (l1 ++ l2) =
-    (string_of_list_ascii l1 ++ string_of_list_ascii l2)%string.
-Proof.
-  revert l2. induction l1; i; s; eauto.
-  rewrite IHl1. eauto.
-Qed.
+(* Lemma string_of_list_ascii_app l1 l2: *)
+(*   string_of_list_ascii (l1 ++ l2) = *)
+(*     (string_of_list_ascii l1 ++ string_of_list_ascii l2)%string. *)
+(* Proof. *)
+(*   revert l2. induction l1; i; s; eauto. *)
+(*   rewrite IHl1. eauto. *)
+(* Qed. *)
 
 (* Lemma string_app_nil s: *)
 (*   (s ++ "")%string = s. *)
@@ -216,128 +191,148 @@ Qed.
 (* Definition name_prefix (i: nat) (name: string) := *)
 (*   HexString.of_nat i +:+ ":" +:+ name. *)
 
-  Lemma string_of_nat_prefix_eq idx1 idx2 method1 method2
-    (EQ: (HexString.of_nat idx1 ++ "." ++ method1 =
-          HexString.of_nat idx2 ++ "." ++ method2)%string)
-    :
-    idx1 = idx2.
-  Proof.
-  Admitted.
+  (* Lemma string_of_nat_prefix_eq idx1 idx2 method1 method2 *)
+  (*   (EQ: (HexString.of_nat idx1 ++ "." ++ method1 = *)
+  (*         HexString.of_nat idx2 ++ "." ++ method2)%string) *)
+  (*   : *)
+  (*   idx1 = idx2. *)
+  (* Proof. *)
+  (* Admitted. *)
 
-  Lemma cell_name_neq idx idx' method
-    (NEQ: idx ≠ idx') sk
-    :
-    alist_find (CellName.mk idx method) (List.map HModSem.trans_r
-      (HModSem.fnsems (HMod.get_modsem (CellA.t idx' StbA) sk))) = None.
-  Proof.
-    unfold CellA.t. unseal "ccr". s.
-    unfold rel_dec, Dec_RelDec, sumbool_to_bool, dec, string_Dec.
-    des_ifs; exfalso; apply string_of_nat_prefix_eq in H1; ss.
-  Qed.
+  (* Lemma cell_name_neq idx idx' method *)
+  (*   (NEQ: idx ≠ idx') sk *)
+  (*   : *)
+  (*   alist_find (CellName.mk idx method) (List.map HModSem.trans_r *)
+  (*     (HModSem.fnsems (HMod.get_modsem (CellA.t idx' StbA) sk))) = None. *)
+  (* Proof. *)
+  (*   unfold CellA.t. unseal "ccr". s. *)
+  (*   unfold rel_dec, Dec_RelDec, sumbool_to_bool, dec, string_Dec. *)
+  (*   des_ifs; exfalso; apply string_of_nat_prefix_eq in H1; ss. *)
+  (* Qed. *)
 
-  Fixpoint emb_rec n fns :=
-    match n with
-    | 0 => List.map HModSem.trans_l fns
-    | S n' => List.map HModSem.trans_r (emb_rec n' fns)
-    end.
+  (* Fixpoint emb_rec n fns := *)
+  (*   match n with *)
+  (*   | 0 => List.map HModSem.trans_l fns *)
+  (*   | S n' => List.map HModSem.trans_r (emb_rec n' fns) *)
+  (*   end. *)
   
-  Lemma cell_name_find max idx method
-    (LT: idx < max) sk
-    :
-    alist_find (CellName.mk idx method) (List.map HModSem.trans_r
-      (HModSem.fnsems (HMod.get_modsem (CellGroup max) sk)))
-    =
-    alist_find (CellName.mk idx method) (List.map HModSem.trans_r
-      (HModSem.fnsems (HMod.get_modsem (CellA.t idx StbA) sk))).
-  Proof.
-    revert_until max. clear -max. induction max; i.
-    { nia. }
-    assert (idx = max \/ idx < max) by nia. des; subst.
-    { s. unfold HModSem.add_fnsems. rewrite List.map_app.
-      destruct (alist_find (CellName.mk max method)
-                  (List.map HModSem.trans_r
-                     (HModSem.fnsems (HMod.get_modsem (CellA.t max StbA) sk)))) eqn: EQ.
-      - eapply alist_find_app. rewrite List.map_map.
+  (* Lemma cell_name_find max idx method *)
+  (*   (LT: idx < max) sk *)
+  (*   : *)
+  (*   alist_find (CellName.mk idx method) (List.map HModSem.trans_r *)
+  (*     (HModSem.fnsems (HMod.get_modsem (CellGroup max) sk))) *)
+  (*   = *)
+  (*   alist_find (CellName.mk idx method) (List.map HModSem.trans_r *)
+  (*     (HModSem.fnsems (HMod.get_modsem (CellA.t idx StbA) sk))). *)
+  (* Proof. *)
+  (*   revert_until max. clear -max. induction max; i. *)
+  (*   { nia. } *)
+  (*   assert (idx = max \/ idx < max) by nia. des; subst. *)
+  (*   { s. unfold HModSem.add_fnsems. rewrite List.map_app. *)
+  (*     destruct (alist_find (CellName.mk max method) *)
+  (*                 (List.map HModSem.trans_r *)
+  (*                    (HModSem.fnsems (HMod.get_modsem (CellA.t max StbA) sk)))) eqn: EQ. *)
+  (*     - eapply alist_find_app. rewrite List.map_map. *)
         
-        Search alist_find.
+  (*       Search alist_find. *)
 
 
 
-      unfold CellA.t. unseal "ccr".
-  match goal with [|-context[alist_find ?x]] => rewrite <-(Seal.sealing_eq "_tmp_" x) end.
-  s; unfold rel_dec, Dec_RelDec, sumbool_to_bool, dec, string_Dec;
-  des_ifs; unseal "_tmp_".
-  + exfalso. inv e.
-    apply (f_equal list_ascii_of_string) in H1.
-    rewrite !list_ascii_of_string_app in H1.
-    apply (f_equal (@rev _)) in H1.
-    rewrite !rev_app_distr in H1.
-    apply app_inv_head in H1.
-    apply (f_equal (@rev _)) in H1.
-    rewrite !rev_involutive in H1.
-    apply (f_equal string_of_list_ascii) in H1.
-    rewrite !string_of_list_ascii_of_string in H1.
-    apply (f_equal HexString.to_nat) in H1.
-    rewrite !HexString.to_nat_of_nat in H1. nia.
-  + exfalso. inv e.
-    apply (f_equal list_ascii_of_string) in H1.
-    rewrite !list_ascii_of_string_app in H1.
-    apply (f_equal (@rev _)) in H1.
-    rewrite !rev_app_distr in H1. ss.
-  +
+  (*     unfold CellA.t. unseal "ccr". *)
+  (* match goal with [|-context[alist_find ?x]] => rewrite <-(Seal.sealing_eq "_tmp_" x) end. *)
+  (* s; unfold rel_dec, Dec_RelDec, sumbool_to_bool, dec, string_Dec; *)
+  (* des_ifs; unseal "_tmp_". *)
+  (* + exfalso. inv e. *)
+  (*   apply (f_equal list_ascii_of_string) in H1. *)
+  (*   rewrite !list_ascii_of_string_app in H1. *)
+  (*   apply (f_equal (@rev _)) in H1. *)
+  (*   rewrite !rev_app_distr in H1. *)
+  (*   apply app_inv_head in H1. *)
+  (*   apply (f_equal (@rev _)) in H1. *)
+  (*   rewrite !rev_involutive in H1. *)
+  (*   apply (f_equal string_of_list_ascii) in H1. *)
+  (*   rewrite !string_of_list_ascii_of_string in H1. *)
+  (*   apply (f_equal HexString.to_nat) in H1. *)
+  (*   rewrite !HexString.to_nat_of_nat in H1. nia. *)
+  (* + exfalso. inv e. *)
+  (*   apply (f_equal list_ascii_of_string) in H1. *)
+  (*   rewrite !list_ascii_of_string_app in H1. *)
+  (*   apply (f_equal (@rev _)) in H1. *)
+  (*   rewrite !rev_app_distr in H1. ss. *)
+  (* + *)
     
 
-    Search string.
+  (*   Search string. *)
 
 
-    Require Import HexString.
+  (*   Require Import HexString. *)
 
 
-    apply string_app_inv_r in H1.
-    apply (f_equal HexString.to_nat) in H1.
-    rewrite !HexString.to_nat_of_nat in H1. nia.
-
-    
-  
-  
-
-  apply string_app_inv in H1.
-  
-  try match goal with [H: @eq string _ _|-_] => inv_string H end.
-
-
-
-  
-  repeat match goal with [H: not (@eq string _ _)|-_] => clear H end
-    
-    destruct idx.
-    -
+  (*   apply string_app_inv_r in H1. *)
+  (*   apply (f_equal HexString.to_nat) in H1. *)
+  (*   rewrite !HexString.to_nat_of_nat in H1. nia. *)
 
     
-    - destruct max_size eqn: EQ; try nia. s. rewrite EQ.
-      unfold CellA.t. unseal "ccr".
+  
+  
 
-  match goal with [|-context[alist_find ?x]] => rewrite <-(Seal.sealing_eq "_tmp_" x) end.
-  s; unfold rel_dec, Dec_RelDec, sumbool_to_bool, dec, string_Dec.
-  des_ifs; unseal "_tmp_".
+  (* apply string_app_inv in H1. *)
+  
+  (* try match goal with [H: @eq string _ _|-_] => inv_string H end. *)
+
+
+
+  
+  (* repeat match goal with [H: not (@eq string _ _)|-_] => clear H end *)
+    
+  (*   destruct idx. *)
+  (*   - *)
+
+    
+  (*   - destruct max_size eqn: EQ; try nia. s. rewrite EQ. *)
+  (*     unfold CellA.t. unseal "ccr". *)
+
+  (* match goal with [|-context[alist_find ?x]] => rewrite <-(Seal.sealing_eq "_tmp_" x) end. *)
+  (* s; unfold rel_dec, Dec_RelDec, sumbool_to_bool, dec, string_Dec. *)
+  (* des_ifs; unseal "_tmp_". *)
 
   
 
   
   
-  repeat match goal with [H: @eq string _ _|-_] => inv_string H end.
+  (* repeat match goal with [H: @eq string _ _|-_] => inv_string H end. *)
 
 
   
-  repeat match goal with [H: not (@eq string _ _)|-_] => clear H end.
+  (* repeat match goal with [H: not (@eq string _ _)|-_] => clear H end. *)
       
-      alist_find_solver.
+  (*     alist_find_solver. *)
       
       
     
     
-  Qed.
+  (* Qed. *)
 
+  Definition rotate_rev {T} n (l: list T) :=
+    drop ((strings.length l)-(n mod strings.length l)) l ++ take ((strings.length l)-(n mod strings.length l)) l.
+
+  Lemma rotate_rev_inv {T} n (l: list T):
+    rotate_rev n (rotate n l) = l.
+  Proof. admit. Admitted.
+
+  Lemma rotate_rev_id {T} (l: list T):
+    rotate_rev 0 l = l.
+  Proof. admit. Admitted.
+  
+  Definition Ist: Any.t -> Any.t -> iProp :=
+    (fun st_src st_tgt =>
+       ((∃ (sz:nat) (q q': list Z) (hd tl: nat) cell_state,
+         ⌜st_src = (sz, q)↑ /\ List.length q = sz /\ sz < max_size /\
+          st_tgt = Any.pair (hd,tl)↑ cell_state /\ hd-tl = sz /\
+          List.length (q ++ q') = max_size⌝ ∗
+          [∗ list] i↦x ∈ rotate_rev tl (q++q'), (CellAS.pending i ∨ CellAS.cell (i mod max_size) x))))%I.
+
+  
   Lemma simF_init:
     HModR.sim_fun RingAMod RingIMod Ist RingName.init.
   Proof.
@@ -359,55 +354,55 @@ Qed.
     admit.
   Admitted.
 
-  Lemma simF_dequeue:
-    HModR.sim_fun RingAMod RingIMod Ist RingName.dequeue.
-  Proof.
-    init_simF.
+(*   Lemma simF_dequeue: *)
+(*     HModR.sim_fun RingAMod RingIMod Ist RingName.dequeue. *)
+(*   Proof. *)
+(*     init_simF. *)
 
-    st_l. iDestruct "ASM" as "%". subst. hss.
-    iDestruct "IST" as (sz q q' hd tl cell_state) "(% & CS)". des; subst.
-    st_l. st_r. hss. rewrite <-H4. destruct (hd-tl) eqn: EQ; s.
-    { st. do 2 force_l. iSplitL ""; eauto.
-      st. iSplitL; eauto. unfold Ist.
-      iExists _,_,_,_,_,_. iFrame.
-      iPureIntro. esplits; eauto. nia.
-    }
+(*     st_l. iDestruct "ASM" as "%". subst. hss. *)
+(*     iDestruct "IST" as (sz q q' hd tl cell_state) "(% & CS)". des; subst. *)
+(*     st_l. st_r. hss. rewrite <-H4. destruct (hd-tl) eqn: EQ; s. *)
+(*     { st. do 2 force_l. iSplitL ""; eauto. *)
+(*       st. iSplitL; eauto. unfold Ist. *)
+(*       iExists _,_,_,_,_,_. iFrame. *)
+(*       iPureIntro. esplits; eauto. nia. *)
+(*     } *)
 
-    st_r.
-    inline_r.
-    { unfold CtrlIMod. unseal "ccr". hide_evars.
-      alist_find_solver. show_evars.
+(*     st_r. *)
+(*     inline_r. *)
+(*     { unfold CtrlIMod. unseal "ccr". hide_evars. *)
+(*       alist_find_solver. show_evars. *)
       
       
 
-  match goal with [|-context[alist_find ?x]] => rewrite <-(Seal.sealing_eq "_tmp_" x) end.
-  s; unfold rel_dec, Dec_RelDec, sumbool_to_bool, dec, string_Dec.
-  des_ifs. unseal "_tmp_".
-  repeat match goal with [H: @eq string _ _|-_] => inv_string H end;
-  repeat match goal with [H: not (@eq string _ _)|-_] => clear H end      
-      alist_find_solver.
+(*   match goal with [|-context[alist_find ?x]] => rewrite <-(Seal.sealing_eq "_tmp_" x) end. *)
+(*   s; unfold rel_dec, Dec_RelDec, sumbool_to_bool, dec, string_Dec. *)
+(*   des_ifs. unseal "_tmp_". *)
+(*   repeat match goal with [H: @eq string _ _|-_] => inv_string H end; *)
+(*   repeat match goal with [H: not (@eq string _ _)|-_] => clear H end       *)
+(*       alist_find_solver. *)
 
       
-  Smatch goal with [|-context[alist_find ?x]] => rewrite <-(Seal.sealing_eq "_tmp_" x) end.
-  s; unfold rel_dec, Dec_RelDec, sumbool_to_bool, dec, string_Dec.
-  des_ifs; unseal "_tmp_".
+(*   Smatch goal with [|-context[alist_find ?x]] => rewrite <-(Seal.sealing_eq "_tmp_" x) end. *)
+(*   s; unfold rel_dec, Dec_RelDec, sumbool_to_bool, dec, string_Dec. *)
+(*   des_ifs; unseal "_tmp_". *)
   
-  repeat match goal with [H: @eq string _ _|-_] => inv_string H end.
-  repeat match goal with [H: @eq string _ _|-_] => inv_string H end.
-  repeat match goal with [H: @eq string _ _|-_] => inv_string H end.
-  repeat match goal with [H: @eq string _ _|-_] => inv_string H end.
+(*   repeat match goal with [H: @eq string _ _|-_] => inv_string H end. *)
+(*   repeat match goal with [H: @eq string _ _|-_] => inv_string H end. *)
+(*   repeat match goal with [H: @eq string _ _|-_] => inv_string H end. *)
+(*   repeat match goal with [H: @eq string _ _|-_] => inv_string H end. *)
 
   
 
   
-  repeat match goal with [H: (_: string) ≠ _|-_] => clear H end.
+(*   repeat match goal with [H: (_: string) ≠ _|-_] => clear H end. *)
 
       
 
 
     
     
-exfalso.
+(* exfalso. *)
 
 
 
@@ -416,53 +411,53 @@ exfalso.
 
 
 
-    force_l. st_l. force_l.
-    iSplitL "". { eauto. }
+(*     force_l. st_l. force_l. *)
+(*     iSplitL "". { eauto. } *)
     
-    st_l. iDestruct "ASM" as "((% & C) & %)".
-    subst. hss. rename y0 into v. unfold Ist.
-    iDestruct "IST" as "[(C0 & _)|(P & IST)]".
-    { iExFalso. iApply (cell_unique with "C0 C"). }
-    iDestruct "IST" as (v') "(A & %)". subst. hss.
+(*     st_l. iDestruct "ASM" as "((% & C) & %)". *)
+(*     subst. hss. rename y0 into v. unfold Ist. *)
+(*     iDestruct "IST" as "[(C0 & _)|(P & IST)]". *)
+(*     { iExFalso. iApply (cell_unique with "C0 C"). } *)
+(*     iDestruct "IST" as (v') "(A & %)". subst. hss. *)
 
-    iPoseProof (cell_auth_get with "C A") as "%". subst.
+(*     iPoseProof (cell_auth_get with "C A") as "%". subst. *)
 
-    st_r. force_l. st_l. force_l. force_l.
-    iSplitL "C". { eauto. }
+(*     st_r. force_l. st_l. force_l. force_l. *)
+(*     iSplitL "C". { eauto. } *)
 
-    st. iSplitL; [|eauto].
-    iRight. iFrame. eauto.
-  Qed.
+(*     st. iSplitL; [|eauto]. *)
+(*     iRight. iFrame. eauto. *)
+(*   Qed. *)
   
-  Lemma simF_set:
-    HModR.sim_fun CellAMod CellIMod Ist (CellName.set idx).
-  Proof.
-    init_simF.
+(*   Lemma simF_set: *)
+(*     HModR.sim_fun CellAMod CellIMod Ist (CellName.set idx). *)
+(*   Proof. *)
+(*     init_simF. *)
     
-    st_l. hss. iDestruct "ASM" as "((% & C) & %)".
-    subst. hss. rename y1 into v, y2 into v0. unfold Ist.
-    iDestruct "IST" as "[(C0 & _)|(P & IST)]".
-    { iExFalso. iApply (cell_unique with "C0 C"). }
-    iDestruct "IST" as (v') "(A & %)". subst. hss.
+(*     st_l. hss. iDestruct "ASM" as "((% & C) & %)". *)
+(*     subst. hss. rename y1 into v, y2 into v0. unfold Ist. *)
+(*     iDestruct "IST" as "[(C0 & _)|(P & IST)]". *)
+(*     { iExFalso. iApply (cell_unique with "C0 C"). } *)
+(*     iDestruct "IST" as (v') "(A & %)". subst. hss. *)
 
-    iPoseProof (cell_auth_get with "C A") as "%". subst.
-    iMod (cell_auth_set with "C A") as "(C & A)".
+(*     iPoseProof (cell_auth_get with "C A") as "%". subst. *)
+(*     iMod (cell_auth_set with "C A") as "(C & A)". *)
     
-    st_r. force_l. st_l. force_l. force_l.
-    iSplitL "C". { eauto. }
+(*     st_r. force_l. st_l. force_l. force_l. *)
+(*     iSplitL "C". { eauto. } *)
 
-    st. iSplitL; [|eauto].
-    iRight. iFrame. eauto.
-  Qed.
+(*     st. iSplitL; [|eauto]. *)
+(*     iRight. iFrame. eauto. *)
+(*   Qed. *)
 
-  Theorem sim: HModR.sim CellAMod CellIMod Ist.
-  Proof.
-    init_sim.
-    - unfold Ist. eauto.
-    - use_simF simF_init.
-    - use_simF simF_get.
-    - use_simF simF_set.
-  Qed.
+(*   Theorem sim: HModR.sim CellAMod CellIMod Ist. *)
+(*   Proof. *)
+(*     init_sim. *)
+(*     - unfold Ist. eauto. *)
+(*     - use_simF simF_init. *)
+(*     - use_simF simF_get. *)
+(*     - use_simF simF_set. *)
+(*   Qed. *)
 
 End SIMMODSEM.
 End RingIA.
