simulations/isim/ISim.v
@@ -52,31 +52,6 @@ End SPEC.
 
 Section LEMMAS.
 
-  Lemma isim_reflR `{Σ: GRA.t} R Ist fnsems_src fnsems_tgt st_src st_tgt (itr: itree _ R):
-    IstProd Ist IstEq st_src st_tgt -∗
-    isim (IstProd Ist IstEq) fnsems_src fnsems_tgt ibot ibot
-    (λ '(st_src, v_src) '(st_tgt, v_tgt), IstProd Ist IstEq st_src st_tgt ** ⌜v_src = v_tgt⌝) false false
-    (st_src, translate (HModSem.emb_ run_r) itr)
-    (st_tgt, translate (HModSem.emb_ run_r) itr).
-  Proof.
-    revert st_src st_tgt. apply combine_quant.
-    revert itr. apply combine_quant.
-  
-    eapply isim_coind. i. destruct a as [itr [st_src st_tgt]]. s.
-    iIntros "(#(_ & CIH) & IST)".
-    assert (CASE := case_itrH _ itr); des; subst.
-    - st. eauto.
-    - st. CIH.
-    - st. force_r. iFrame. CIH.
-    - st. force_l. iFrame. CIH.
-    - destruct c. st. call; eauto. CIH.
-    - destruct s. st.
-      iPoseProof (ist_eq_run_r with "IST") as "(%EQ & IST)". rewrite <-EQ.
-      CIH.
-    - destruct e; st; force_l; force_r; CIH.
-  Qed.
-
-
 (***** Move and rename: APC & HoareCall LEMMAS *****)
 
   (* Try to match bind pattern *)
