simulations/isim/ITactics.v
@@ -15,60 +15,9 @@ Require Import Red IRed.
 Require Import HPSim.
 Require Import World sWorld.
 Require Import ISimCore ITacticsInternal.
-Require Import Events Mod SMod.
+Require Import Events Mod SMod HMod.
 
 From stdpp Require Import coPset gmap.
-
-(* use this to enforce the ssr_reflect rewrite: rewrite/__ rules. *)
-Definition __ : Type := unit.
-
-Lemma string_app_inv
-  p s s'
-  (EQ: (p ++ s = p ++ s')%string)
-  :
-  (s = s')%string.
-Proof.
-  revert_until p. induction p; i; ss.
-  unfold append in EQ. depdes EQ. eauto.
-Qed.
-
-Ltac inv_string X :=
-  inv X;
-  repeat match goal with [H: (_ ++ _)%string = (_ ++ _)%string|-_] =>
-           apply string_app_inv in H
-         end; ss.
-
-Ltac alist_find_solver :=
-  match goal with [|-context[alist_find ?x]] => rewrite <-(Seal.sealing_eq "_tmp_" x) end;
-  s; unfold rel_dec, Dec_RelDec, sumbool_to_bool, dec, string_Dec;
-  des_ifs; unseal "_tmp_";
-  repeat match goal with [H: (_: string) =  _|-_] => inv_string H end;
-  repeat match goal with [H: (_: string) ≠ _|-_] => clear H end.
-
-Ltac init_simF := let name := fresh "name" in
-  match goal with [|-_ ?x ?y _ _] => rewrite /x /y end; unseal "ccr";
-  unfold HModR.sim_fun; i;
-  alist_find_solver;
-  repeat match goal with
-  | [|- context[{| fsb_body := ?x |}]] => rewrite/__ {1}/x
-  | [|- context[cfunU ?x]] => rewrite/__ {1}/x
-  end;
-  unfold interp_sb_hp, HoareFun, cfunU, ccallU; s;
-  ii; subst; iIntros "IST".
-
-Ltac init_sim :=
-  match goal with [|- HModR.sim ?x ?y _] => rewrite /x /y end; unseal "ccr";
-  econs; [|eauto];
-  i; econs; [s|eauto|i; ss; des_ifs|i; ss; des_ifs].
-
-Ltac use_simF lem :=
-  esplits; eauto;
-  assert (X:= lem); revert X;
-  match goal with [|-_ ?x ?y _ _ -> _] => rewrite /x /y end; unseal "ccr";
-  unfold HModR.sim_fun;
-  alist_find_solver.
-
-
 
 (************ User Tactics **************)
 (* Tactic Notation "simF_init" constr(LS) constr(LT) reference(FS) reference(FT) := *)
@@ -80,13 +29,25 @@ Ltac use_simF lem :=
 (* need change *)
 (* Ltac sim_init := econs; eauto; ii; econs; cycle 1; [s|sim_split]. *)
 
+(* use this to enforce the ssr_reflect rewrite: rewrite/__ rules. *)
+Definition __ : Type := unit.
+
+Ltac unfold_hmod :=
+  match goal with
+  | [|-context[HMod.get_modsem ?x _]] => rewrite/__ {1}/x; progress unseal "ccr"
+  | [|-context[HMod.sk ?x]] => rewrite/__ {1}/x; progress unseal "ccr" end.
+
+(***
+  Step-level tactics
+ ***)
+
 Ltac st := repeat _st.
 
 Ltac force_l := try (prep; _force_l).
 Ltac force_r := try (prep; _force_r).
 
-Ltac inline_l := prep; iApply isim_inline_src; [eauto|]; unfold interp_sb_hp, HoareFun.
-Ltac inline_r := prep; iApply isim_inline_tgt; [eauto|]; unfold interp_sb_hp, HoareFun.
+Ltac inline_l := prep; iApply isim_inline_src; [repeat unfold_hmod; eauto|]; unfold interp_sb_hp, HoareFun; s.
+Ltac inline_r := prep; iApply isim_inline_tgt; [repeat unfold_hmod; eauto|]; unfold interp_sb_hp, HoareFun; s.
 
 Ltac call := prep; iApply isim_call; iSplitL "IST"; [ |iIntros "% % %"; iIntrosFresh "IST"].
 
@@ -109,8 +70,7 @@ Ltac apc_r :=
 
 Ltac hss :=
   ss;
-  try (unfold run_l; rewrite !Any.pair_split; fold run_l);
-  try (unfold run_r; rewrite !Any.pair_split; fold run_r);
+  try (unfold run_l, run_r in *; rewrite !Any.pair_split in *; fold run_l run_r in * );
   try (rewrite !Any.upcast_downcast in * );
   (repeat match goal with [G: Any.downcast _ = Some _ |-_] =>
     apply Any.downcast_upcast in G; inv G; ss
@@ -145,6 +105,101 @@ iApply isim_progress; iApply isim_base;
 match goal with [|- context[_ ?R _ _ _ (?st_src, _ _ ?itr) (?st_tgt, _)]] =>
   iApply ("CIH" $! (@existT _ (λ _, _) itr (@existT _ (λ _, _) st_src st_tgt))); eauto
 end.
+
+(***
+ Module-level tactics
+ ***)
+
+Lemma string_app_inv
+  p s s'
+  (EQ: (p ++ s = p ++ s')%string)
+  :
+  (s = s')%string.
+Proof.
+  revert_until p. induction p; i; ss.
+  unfold append in EQ. depdes EQ. eauto.
+Qed.
+
+Lemma isim_reflR `{Σ: GRA.t} R Ist fnsems_src fnsems_tgt st_src st_tgt (itr: itree _ R):
+  IstProd Ist IstEq st_src st_tgt -∗
+  isim (IstProd Ist IstEq) fnsems_src fnsems_tgt ibot ibot
+  (λ '(st_src, v_src) '(st_tgt, v_tgt), IstProd Ist IstEq st_src st_tgt ** ⌜v_src = v_tgt⌝) false false
+  (st_src, translate (HModSem.emb_ run_r) itr)
+  (st_tgt, translate (HModSem.emb_ run_r) itr).
+Proof.
+  revert st_src st_tgt. apply combine_quant.
+  revert itr. apply combine_quant.
+
+  eapply isim_coind. i. destruct a as [itr [st_src st_tgt]]. s.
+  iIntros "(#(_ & CIH) & IST)".
+  assert (CASE := case_itrH _ itr); des; subst.
+  - st. eauto.
+  - st. CIH.
+  - st. force_r. iFrame. CIH.
+  - st. force_l. iFrame. CIH.
+  - destruct c. st. call; eauto. CIH.
+  - destruct s. st.
+    iPoseProof (ist_eq_run_r with "IST") as "(%EQ & IST)". rewrite <-EQ.
+    CIH.
+  - destruct e; st; force_l; force_r; CIH.
+Qed.
+
+Ltac inv_string X :=
+  inv X;
+  repeat match goal with [H: @eq string (_ ++ _)%string (_ ++ _)%string|-_] =>
+           apply string_app_inv in H
+    end; ss.
+
+Ltac alist_find_solver :=
+  match goal with [|-context[alist_find ?x]] => rewrite <-(Seal.sealing_eq "_tmp_" x) end;
+  s; unfold rel_dec, Dec_RelDec, sumbool_to_bool, dec, string_Dec;
+  des_ifs; unseal "_tmp_"; ss;
+  repeat match goal with [H: @eq string _ _|-_] => inv_string H end;
+  repeat match goal with [H: not (@eq string _ _)|-_] => clear H end.
+
+Ltac init_simF := let TMP := fresh "_tmp_" in
+  unfold HModR.sim_fun; i; s;
+  unfold_hmod;
+  match goal with [|-context[alist_find _ ?x]] =>
+    set (TMP := x); unfold_hmod; unfold TMP; clear TMP
+  end;
+  alist_find_solver;
+  repeat match goal with
+  | [|- context[{| fsb_body := cfunU ?x |}]] => rewrite/__ {1}/x
+  | [|- context[{| fsb_body := ?x |}]] => rewrite/__ {1}/x
+  | [|- context[cfunU ?x]] => rewrite/__ {1}/x
+  end;
+  unfold interp_sb_hp, HoareFun, cfunU, ccallU; s;
+  ii; subst; iIntros "IST".
+
+Ltac init_sim := let TMP := fresh "_tmp_" in
+  econs; s;
+  [econs; [repeat unfold_hmod;ss|repeat unfold_hmod;ss|
+           repeat unfold_hmod;ss; i; des_ifs|
+    s; i; des_ifs;
+    match goal with [H:_|-_] => revert H end;
+    unfold_hmod;
+    match goal with [|-context[alist_find _ ?x]] =>
+      set (TMP := x); unfold_hmod; unfold TMP; clear TMP
+    end;
+    alist_find_solver]
+  |repeat unfold_hmod; ss].
+
+Ltac use_simF lem := let TMP := fresh "_tmp_" in
+  intros TMP; inv TMP;
+  esplits; eauto;
+  eassert (X:= lem _); revert X; s;
+  unfold_hmod;
+  match goal with [|-context[alist_find _ ?x]] =>
+    set (TMP := x); unfold_hmod; unfold TMP; clear TMP
+  end;
+  alist_find_solver; eauto.
+
+Ltac refl_simF := let TMP := fresh "_tmp_" in
+  repeat unfold_hmod;
+  alist_find_solver; intros TMP; inv TMP; esplits; eauto;
+  ii; subst; eapply isim_reflR.
+
 
 
 
